<?xml version="1.0"?>
<rdf:RDF xmlns="http://www.semanticweb.org/abc/ontologies/2025/3/untitled-ontology-11#"
     xml:base="http://www.semanticweb.org/abc/ontologies/2025/3/untitled-ontology-11"
     xmlns:owl="http://www.w3.org/2002/07/owl#"
     xmlns:rdf="http://www.w3.org/1999/02/22-rdf-syntax-ns#"
     xmlns:xml="http://www.w3.org/XML/1998/namespace"
     xmlns:xsd="http://www.w3.org/2001/XMLSchema#"
     xmlns:rdfs="http://www.w3.org/2000/01/rdf-schema#">
    <owl:Ontology rdf:about="http://www.semanticweb.org/abc/ontologies/2025/3/untitled-ontology-11"/>
    


    <!-- 
    ///////////////////////////////////////////////////////////////////////////////////////
    //
    // Datatypes
    //
    ///////////////////////////////////////////////////////////////////////////////////////
     -->

    


    <!-- http://schema.org/contentSize -->

    <rdfs:Datatype rdf:about="http://schema.org/contentSize"/>
    


    <!-- http://schema.org/dateModified -->

    <rdfs:Datatype rdf:about="http://schema.org/dateModified"/>
    


    <!-- http://schema.org/dateSubmitted -->

    <rdfs:Datatype rdf:about="http://schema.org/dateSubmitted"/>
    


    <!-- http://schema.org/department -->

    <rdfs:Datatype rdf:about="http://schema.org/department"/>
    


    <!-- http://schema.org/description -->

    <rdfs:Datatype rdf:about="http://schema.org/description"/>
    


    <!-- http://schema.org/duration -->

    <rdfs:Datatype rdf:about="http://schema.org/duration"/>
    


    <!-- http://schema.org/email -->

    <rdfs:Datatype rdf:about="http://schema.org/email"/>
    


    <!-- http://schema.org/encodingformat -->

    <rdfs:Datatype rdf:about="http://schema.org/encodingformat"/>
    


    <!-- http://schema.org/endDate -->

    <rdfs:Datatype rdf:about="http://schema.org/endDate"/>
    


    <!-- http://schema.org/identifier -->

    <rdfs:Datatype rdf:about="http://schema.org/identifier"/>
    


    <!-- http://schema.org/jobTitle -->

    <rdfs:Datatype rdf:about="http://schema.org/jobTitle"/>
    


    <!-- http://schema.org/license -->

    <rdfs:Datatype rdf:about="http://schema.org/license"/>
    


    <!-- http://schema.org/name -->

    <rdfs:Datatype rdf:about="http://schema.org/name"/>
    


    <!-- http://schema.org/programmingLanguage -->

    <rdfs:Datatype rdf:about="http://schema.org/programmingLanguage"/>
    


    <!-- http://schema.org/roleName -->

    <rdfs:Datatype rdf:about="http://schema.org/roleName"/>
    


    <!-- http://schema.org/softwareFramework -->

    <rdfs:Datatype rdf:about="http://schema.org/softwareFramework"/>
    


    <!-- http://schema.org/startDate -->

    <rdfs:Datatype rdf:about="http://schema.org/startDate"/>
    


    <!-- http://schema.org/telephone -->

    <rdfs:Datatype rdf:about="http://schema.org/telephone"/>
    


    <!-- http://schema.org/version -->

    <rdfs:Datatype rdf:about="http://schema.org/version"/>
    


    <!-- http://schema.org/videoFrameSize -->

    <rdfs:Datatype rdf:about="http://schema.org/videoFrameSize"/>
    


    <!-- http://schema.org/videoQuality -->

    <rdfs:Datatype rdf:about="http://schema.org/videoQuality"/>
    


    <!-- 
    ///////////////////////////////////////////////////////////////////////////////////////
    //
    // Object Properties
    //
    ///////////////////////////////////////////////////////////////////////////////////////
     -->

    


    <!-- http://schema.org/creator -->

    <owl:ObjectProperty rdf:about="http://schema.org/creator">
        <rdfs:domain rdf:resource="http://www.semanticweb.org/abc/ontologies/2025/3/untitled-ontology-11#Student"/>
        <rdfs:range>
            <owl:Class>
                <owl:unionOf rdf:parseType="Collection">
                    <rdf:Description rdf:about="http://www.semanticweb.org/abc/ontologies/2025/3/untitled-ontology-11#Documentation"/>
                    <rdf:Description rdf:about="http://www.semanticweb.org/abc/ontologies/2025/3/untitled-ontology-11#Poster"/>
                    <rdf:Description rdf:about="http://www.semanticweb.org/abc/ontologies/2025/3/untitled-ontology-11#Proposal"/>
                    <rdf:Description rdf:about="http://www.semanticweb.org/abc/ontologies/2025/3/untitled-ontology-11#Video"/>
                </owl:unionOf>
            </owl:Class>
        </rdfs:range>
        <rdfs:comment>This element represents the concept of &apos;creator&apos; as used in the capstone project ontology.</rdfs:comment>
        <rdfs:label>creator</rdfs:label>
    </owl:ObjectProperty>
    


    <!-- http://schema.org/isPartOf -->

    <owl:ObjectProperty rdf:about="http://schema.org/isPartOf">
        <owl:inverseOf rdf:resource="http://www.semanticweb.org/abc/ontologies/2025/3/untitled-ontology-11#hasComponent"/>
        <rdfs:domain rdf:resource="http://www.semanticweb.org/abc/ontologies/2025/3/untitled-ontology-11#ProjectComponent"/>
        <rdfs:range rdf:resource="http://www.semanticweb.org/abc/ontologies/2025/3/untitled-ontology-11#CapstoneProject"/>
        <rdfs:comment>This element represents the concept of &apos;isPartOf&apos; as used in the capstone project ontology.</rdfs:comment>
        <rdfs:label>isPartOf</rdfs:label>
    </owl:ObjectProperty>
    


    <!-- http://www.semanticweb.org/abc/ontologies/2025/3/untitled-ontology-11#evaluatedBy -->

    <owl:ObjectProperty rdf:about="http://www.semanticweb.org/abc/ontologies/2025/3/untitled-ontology-11#evaluatedBy">
        <rdfs:domain rdf:resource="http://www.semanticweb.org/abc/ontologies/2025/3/untitled-ontology-11#Evaluation"/>
        <rdfs:range rdf:resource="http://www.semanticweb.org/abc/ontologies/2025/3/untitled-ontology-11#Stakeholder"/>
        <rdfs:comment>This element represents the concept of &apos;evaluatedBy&apos; as used in the capstone project ontology.</rdfs:comment>
        <rdfs:label>evaluatedBy</rdfs:label>
    </owl:ObjectProperty>
    


    <!-- http://www.semanticweb.org/abc/ontologies/2025/3/untitled-ontology-11#evaluatesBasedOnCriteria -->

    <owl:ObjectProperty rdf:about="http://www.semanticweb.org/abc/ontologies/2025/3/untitled-ontology-11#evaluatesBasedOnCriteria">
        <rdfs:domain rdf:resource="http://www.semanticweb.org/abc/ontologies/2025/3/untitled-ontology-11#Evaluation"/>
        <rdfs:range rdf:resource="http://www.semanticweb.org/abc/ontologies/2025/3/untitled-ontology-11#Criteria"/>
        <rdfs:comment>This element represents the concept of &apos;evaluatesBasedOnCriteria&apos; as used in the capstone project ontology.</rdfs:comment>
        <rdfs:label>evaluatesBasedOnCriteria</rdfs:label>
    </owl:ObjectProperty>
    


    <!-- http://www.semanticweb.org/abc/ontologies/2025/3/untitled-ontology-11#hasComponent -->

    <owl:ObjectProperty rdf:about="http://www.semanticweb.org/abc/ontologies/2025/3/untitled-ontology-11#hasComponent">
        <rdfs:domain rdf:resource="http://www.semanticweb.org/abc/ontologies/2025/3/untitled-ontology-11#CapstoneProject"/>
        <rdfs:range rdf:resource="http://www.semanticweb.org/abc/ontologies/2025/3/untitled-ontology-11#ProjectComponent"/>
        <rdfs:comment>This element represents the concept of &apos;hasComponent&apos; as used in the capstone project ontology.</rdfs:comment>
        <rdfs:label>hasComponent</rdfs:label>
    </owl:ObjectProperty>
    


    <!-- http://www.semanticweb.org/abc/ontologies/2025/3/untitled-ontology-11#hasPosterTool -->

    <owl:ObjectProperty rdf:about="http://www.semanticweb.org/abc/ontologies/2025/3/untitled-ontology-11#hasPosterTool">
        <rdfs:domain rdf:resource="http://www.semanticweb.org/abc/ontologies/2025/3/untitled-ontology-11#Poster"/>
        <rdfs:range rdf:resource="http://www.semanticweb.org/abc/ontologies/2025/3/untitled-ontology-11#Postertool"/>
        <rdfs:comment>This element represents the concept of &apos;hasPosterTool&apos; as used in the capstone project ontology.</rdfs:comment>
        <rdfs:label>hasPosterTool</rdfs:label>
    </owl:ObjectProperty>
    


    <!-- http://www.semanticweb.org/abc/ontologies/2025/3/untitled-ontology-11#hasProcess -->

    <owl:ObjectProperty rdf:about="http://www.semanticweb.org/abc/ontologies/2025/3/untitled-ontology-11#hasProcess">
        <rdfs:domain rdf:resource="http://www.semanticweb.org/abc/ontologies/2025/3/untitled-ontology-11#CapstoneProject"/>
        <rdfs:range rdf:resource="http://www.semanticweb.org/abc/ontologies/2025/3/untitled-ontology-11#Process"/>
        <rdfs:comment>This element represents the concept of &apos;hasProcess&apos; as used in the capstone project ontology.</rdfs:comment>
        <rdfs:label>hasProcess</rdfs:label>
    </owl:ObjectProperty>
    


    <!-- http://www.semanticweb.org/abc/ontologies/2025/3/untitled-ontology-11#hasProposalTool -->

    <owl:ObjectProperty rdf:about="http://www.semanticweb.org/abc/ontologies/2025/3/untitled-ontology-11#hasProposalTool">
        <rdfs:domain rdf:resource="http://www.semanticweb.org/abc/ontologies/2025/3/untitled-ontology-11#Proposal"/>
        <rdfs:range rdf:resource="http://www.semanticweb.org/abc/ontologies/2025/3/untitled-ontology-11#Proposaltool"/>
        <rdfs:comment>This element represents the concept of  &apos;hasProposalTool&apos; as used in the capstone project ontology.</rdfs:comment>
        <rdfs:label>hasProposalTool</rdfs:label>
    </owl:ObjectProperty>
    


    <!-- http://www.semanticweb.org/abc/ontologies/2025/3/untitled-ontology-11#hasStakeholder -->

    <owl:ObjectProperty rdf:about="http://www.semanticweb.org/abc/ontologies/2025/3/untitled-ontology-11#hasStakeholder">
        <rdfs:domain rdf:resource="http://www.semanticweb.org/abc/ontologies/2025/3/untitled-ontology-11#CapstoneProject"/>
        <rdfs:range rdf:resource="http://www.semanticweb.org/abc/ontologies/2025/3/untitled-ontology-11#Stakeholder"/>
        <rdfs:comment>This element represents the concept of &apos;hasStakeholder&apos; as used in the capstone project ontology.</rdfs:comment>
        <rdfs:label>hasStakeholder</rdfs:label>
    </owl:ObjectProperty>
    


    <!-- http://www.semanticweb.org/abc/ontologies/2025/3/untitled-ontology-11#hasTool -->

    <owl:ObjectProperty rdf:about="http://www.semanticweb.org/abc/ontologies/2025/3/untitled-ontology-11#hasTool">
        <rdfs:domain rdf:resource="http://www.semanticweb.org/abc/ontologies/2025/3/untitled-ontology-11#CapstoneProject"/>
        <rdfs:range rdf:resource="http://www.semanticweb.org/abc/ontologies/2025/3/untitled-ontology-11#Tools"/>
        <rdfs:comment>This element represents the concept of &apos;hasTool&apos; as used in the capstone project ontology.</rdfs:comment>
        <rdfs:label>hasTool</rdfs:label>
    </owl:ObjectProperty>
    


    <!-- http://www.semanticweb.org/abc/ontologies/2025/3/untitled-ontology-11#hasVideoTool -->

    <owl:ObjectProperty rdf:about="http://www.semanticweb.org/abc/ontologies/2025/3/untitled-ontology-11#hasVideoTool">
        <rdfs:domain rdf:resource="http://www.semanticweb.org/abc/ontologies/2025/3/untitled-ontology-11#Video"/>
        <rdfs:range rdf:resource="http://www.semanticweb.org/abc/ontologies/2025/3/untitled-ontology-11#Videotool"/>
        <rdfs:comment>This element represents the concept of &apos;hasVideoTool&apos; as used in the capstone project ontology.</rdfs:comment>
        <rdfs:label>hasVideoTool</rdfs:label>
    </owl:ObjectProperty>
    


    <!-- http://www.semanticweb.org/abc/ontologies/2025/3/untitled-ontology-11#implementsProcess -->

    <owl:ObjectProperty rdf:about="http://www.semanticweb.org/abc/ontologies/2025/3/untitled-ontology-11#implementsProcess">
        <rdfs:domain rdf:resource="http://www.semanticweb.org/abc/ontologies/2025/3/untitled-ontology-11#Student"/>
        <rdfs:range rdf:resource="http://www.semanticweb.org/abc/ontologies/2025/3/untitled-ontology-11#Process"/>
        <rdfs:comment>This element represents the concept of &apos;implementsProcess&apos; as used in the capstone project ontology.</rdfs:comment>
        <rdfs:label>implementsProcess</rdfs:label>
    </owl:ObjectProperty>
    


    <!-- http://www.semanticweb.org/abc/ontologies/2025/3/untitled-ontology-11#managesProjectComponent -->

    <owl:ObjectProperty rdf:about="http://www.semanticweb.org/abc/ontologies/2025/3/untitled-ontology-11#managesProjectComponent">
        <rdfs:domain rdf:resource="http://www.semanticweb.org/abc/ontologies/2025/3/untitled-ontology-11#Manager"/>
        <rdfs:range rdf:resource="http://www.semanticweb.org/abc/ontologies/2025/3/untitled-ontology-11#ProjectComponent"/>
        <rdfs:comment>This element represents the concept of &apos;managesProjectComponent&apos; as used in the capstone project ontology.</rdfs:comment>
        <rdfs:label>managesProjectComponent</rdfs:label>
    </owl:ObjectProperty>
    


    <!-- http://www.semanticweb.org/abc/ontologies/2025/3/untitled-ontology-11#presentedBy -->

    <owl:ObjectProperty rdf:about="http://www.semanticweb.org/abc/ontologies/2025/3/untitled-ontology-11#presentedBy">
        <rdfs:domain rdf:resource="http://www.semanticweb.org/abc/ontologies/2025/3/untitled-ontology-11#Student"/>
        <rdfs:range rdf:resource="http://www.semanticweb.org/abc/ontologies/2025/3/untitled-ontology-11#Presentation"/>
        <rdfs:comment>This element represents the concept of &apos;presentedBy&apos; as used in the capstone project ontology.</rdfs:comment>
        <rdfs:label>presentedBy</rdfs:label>
    </owl:ObjectProperty>
    


    <!-- http://www.semanticweb.org/abc/ontologies/2025/3/untitled-ontology-11#produces -->

    <owl:ObjectProperty rdf:about="http://www.semanticweb.org/abc/ontologies/2025/3/untitled-ontology-11#produces">
        <rdfs:domain rdf:resource="http://www.semanticweb.org/abc/ontologies/2025/3/untitled-ontology-11#Process"/>
        <rdfs:range rdf:resource="http://www.semanticweb.org/abc/ontologies/2025/3/untitled-ontology-11#Deliverable"/>
        <rdfs:comment>This element represents the concept of &apos;produces&apos; as used in the capstone project ontology.</rdfs:comment>
        <rdfs:label>produces</rdfs:label>
    </owl:ObjectProperty>
    


    <!-- http://www.semanticweb.org/abc/ontologies/2025/3/untitled-ontology-11#requiresTool -->

    <owl:ObjectProperty rdf:about="http://www.semanticweb.org/abc/ontologies/2025/3/untitled-ontology-11#requiresTool">
        <rdfs:domain rdf:resource="http://www.semanticweb.org/abc/ontologies/2025/3/untitled-ontology-11#Implementation"/>
        <rdfs:range rdf:resource="http://www.semanticweb.org/abc/ontologies/2025/3/untitled-ontology-11#Tools"/>
        <rdfs:comment>This element represents the concept of &apos;requiresTool&apos; as used in the capstone project ontology.</rdfs:comment>
        <rdfs:label>requiresTool</rdfs:label>
    </owl:ObjectProperty>
    


    <!-- http://www.semanticweb.org/abc/ontologies/2025/3/untitled-ontology-11#submitsTo -->

    <owl:ObjectProperty rdf:about="http://www.semanticweb.org/abc/ontologies/2025/3/untitled-ontology-11#submitsTo">
        <rdfs:domain rdf:resource="http://www.semanticweb.org/abc/ontologies/2025/3/untitled-ontology-11#Student"/>
        <rdfs:range rdf:resource="http://www.semanticweb.org/abc/ontologies/2025/3/untitled-ontology-11#Manager"/>
        <rdfs:comment>This element represents the concept of &apos;submitsTo&apos; as used in the capstone project ontology.</rdfs:comment>
        <rdfs:label>submitsTo</rdfs:label>
    </owl:ObjectProperty>
    


    <!-- http://www.semanticweb.org/abc/ontologies/2025/3/untitled-ontology-11#supervises -->

    <owl:ObjectProperty rdf:about="http://www.semanticweb.org/abc/ontologies/2025/3/untitled-ontology-11#supervises">
        <rdfs:domain rdf:resource="http://www.semanticweb.org/abc/ontologies/2025/3/untitled-ontology-11#Supervisor"/>
        <rdfs:range rdf:resource="http://www.semanticweb.org/abc/ontologies/2025/3/untitled-ontology-11#Student"/>
        <rdfs:comment>This element represents the concept of &apos;supervises&apos; as used in the capstone project ontology.</rdfs:comment>
        <rdfs:label>supervises</rdfs:label>
    </owl:ObjectProperty>
    


    <!-- http://www.semanticweb.org/abc/ontologies/2025/3/untitled-ontology-11#useTool -->

    <owl:ObjectProperty rdf:about="http://www.semanticweb.org/abc/ontologies/2025/3/untitled-ontology-11#useTool">
        <rdfs:domain rdf:resource="http://www.semanticweb.org/abc/ontologies/2025/3/untitled-ontology-11#Process"/>
        <rdfs:range rdf:resource="http://www.semanticweb.org/abc/ontologies/2025/3/untitled-ontology-11#Tools"/>
        <rdfs:comment>This element represents the concept of &apos;useTool&apos; as used in the capstone project ontology.</rdfs:comment>
        <rdfs:label>useTool</rdfs:label>
    </owl:ObjectProperty>
    


    <!-- 
    ///////////////////////////////////////////////////////////////////////////////////////
    //
    // Data properties
    //
    ///////////////////////////////////////////////////////////////////////////////////////
     -->

    


    <!-- http://www.semanticweb.org/abc/ontologies/2025/3/untitled-ontology-11#aiModelName -->

    <owl:DatatypeProperty rdf:about="http://www.semanticweb.org/abc/ontologies/2025/3/untitled-ontology-11#aiModelName">
        <rdfs:subPropertyOf rdf:resource="http://www.w3.org/2002/07/owl#topDataProperty"/>
        <rdfs:domain rdf:resource="http://www.semanticweb.org/abc/ontologies/2025/3/untitled-ontology-11#AIModel"/>
        <rdfs:range rdf:resource="http://www.w3.org/2001/XMLSchema#string"/>
        <rdfs:comment>This element represents the concept of &apos;aiModelName&apos; as used in the capstone project ontology.</rdfs:comment>
        <rdfs:label>aiModelName</rdfs:label>
    </owl:DatatypeProperty>
    


    <!-- http://www.semanticweb.org/abc/ontologies/2025/3/untitled-ontology-11#aiModelPurpose -->

    <owl:DatatypeProperty rdf:about="http://www.semanticweb.org/abc/ontologies/2025/3/untitled-ontology-11#aiModelPurpose">
        <rdfs:subPropertyOf rdf:resource="http://www.w3.org/2002/07/owl#topDataProperty"/>
        <rdfs:domain rdf:resource="http://www.semanticweb.org/abc/ontologies/2025/3/untitled-ontology-11#AIModel"/>
        <rdfs:range rdf:resource="http://www.w3.org/2001/XMLSchema#string"/>
        <rdfs:comment>This element represents the concept of &apos;aiModelPurpose&apos; as used in the capstone project ontology.</rdfs:comment>
        <rdfs:label>aiModelPurpose</rdfs:label>
    </owl:DatatypeProperty>
    


    <!-- http://www.semanticweb.org/abc/ontologies/2025/3/untitled-ontology-11#criteriaDescription -->

    <owl:DatatypeProperty rdf:about="http://www.semanticweb.org/abc/ontologies/2025/3/untitled-ontology-11#criteriaDescription">
        <rdfs:subPropertyOf rdf:resource="http://www.w3.org/2002/07/owl#topDataProperty"/>
        <rdfs:domain rdf:resource="http://www.semanticweb.org/abc/ontologies/2025/3/untitled-ontology-11#Criteria"/>
        <rdfs:range rdf:resource="http://schema.org/description"/>
        <rdfs:comment>This element represents the concept of &apos;criteriaDescription&apos; as used in the capstone project ontology.</rdfs:comment>
        <rdfs:label>criteriaDescription</rdfs:label>
    </owl:DatatypeProperty>
    


    <!-- http://www.semanticweb.org/abc/ontologies/2025/3/untitled-ontology-11#databaseType -->

    <owl:DatatypeProperty rdf:about="http://www.semanticweb.org/abc/ontologies/2025/3/untitled-ontology-11#databaseType">
        <rdfs:subPropertyOf rdf:resource="http://www.w3.org/2002/07/owl#topDataProperty"/>
        <rdfs:domain rdf:resource="http://www.semanticweb.org/abc/ontologies/2025/3/untitled-ontology-11#Database"/>
        <rdfs:range rdf:resource="http://www.w3.org/2001/XMLSchema#string"/>
        <rdfs:comment>This element represents the concept of &apos;databaseType&apos; as used in the capstone project ontology.</rdfs:comment>
        <rdfs:label>databaseType</rdfs:label>
    </owl:DatatypeProperty>
    


    <!-- http://www.semanticweb.org/abc/ontologies/2025/3/untitled-ontology-11#department -->

    <owl:DatatypeProperty rdf:about="http://www.semanticweb.org/abc/ontologies/2025/3/untitled-ontology-11#department">
        <rdfs:subPropertyOf rdf:resource="http://www.w3.org/2002/07/owl#topDataProperty"/>
        <rdfs:domain rdf:resource="http://www.semanticweb.org/abc/ontologies/2025/3/untitled-ontology-11#Student"/>
        <rdfs:range rdf:resource="http://schema.org/department"/>
        <rdfs:comment>This element represents the concept of &apos;department&apos; as used in the capstone project ontology.</rdfs:comment>
        <rdfs:label>department</rdfs:label>
    </owl:DatatypeProperty>
    


    <!-- http://www.semanticweb.org/abc/ontologies/2025/3/untitled-ontology-11#designation -->

    <owl:DatatypeProperty rdf:about="http://www.semanticweb.org/abc/ontologies/2025/3/untitled-ontology-11#designation">
        <rdfs:subPropertyOf rdf:resource="http://www.w3.org/2002/07/owl#topDataProperty"/>
        <rdfs:domain rdf:resource="http://www.semanticweb.org/abc/ontologies/2025/3/untitled-ontology-11#FacultyMember"/>
        <rdfs:range rdf:resource="http://schema.org/jobTitle"/>
        <rdfs:comment>This element represents the concept of &apos;designation&apos; as used in the capstone project ontology.</rdfs:comment>
        <rdfs:label>designation</rdfs:label>
    </owl:DatatypeProperty>
    


    <!-- http://www.semanticweb.org/abc/ontologies/2025/3/untitled-ontology-11#documentVersion -->

    <owl:DatatypeProperty rdf:about="http://www.semanticweb.org/abc/ontologies/2025/3/untitled-ontology-11#documentVersion">
        <rdfs:subPropertyOf rdf:resource="http://www.w3.org/2002/07/owl#topDataProperty"/>
        <rdfs:domain rdf:resource="http://www.semanticweb.org/abc/ontologies/2025/3/untitled-ontology-11#Documentation"/>
        <rdfs:range rdf:resource="http://schema.org/version"/>
        <rdfs:comment>This element represents the concept of &apos;documentVersion&apos; as used in the capstone project ontology.</rdfs:comment>
        <rdfs:label>documentVersion</rdfs:label>
    </owl:DatatypeProperty>
    


    <!-- http://www.semanticweb.org/abc/ontologies/2025/3/untitled-ontology-11#durationInWeeks -->

    <owl:DatatypeProperty rdf:about="http://www.semanticweb.org/abc/ontologies/2025/3/untitled-ontology-11#durationInWeeks">
        <rdfs:subPropertyOf rdf:resource="http://www.w3.org/2002/07/owl#topDataProperty"/>
        <rdfs:domain rdf:resource="http://www.semanticweb.org/abc/ontologies/2025/3/untitled-ontology-11#CapstoneProject"/>
        <rdfs:range rdf:resource="http://schema.org/duration"/>
        <rdfs:comment>This element represents the concept of &apos;durationInWeeks&apos; as used in the capstone project ontology.</rdfs:comment>
        <rdfs:label>durationInWeeks</rdfs:label>
    </owl:DatatypeProperty>
    


    <!-- http://www.semanticweb.org/abc/ontologies/2025/3/untitled-ontology-11#email -->

    <owl:DatatypeProperty rdf:about="http://www.semanticweb.org/abc/ontologies/2025/3/untitled-ontology-11#email">
        <rdfs:subPropertyOf rdf:resource="http://www.w3.org/2002/07/owl#topDataProperty"/>
        <rdfs:domain rdf:resource="http://www.semanticweb.org/abc/ontologies/2025/3/untitled-ontology-11#Stakeholder"/>
        <rdfs:range rdf:resource="http://schema.org/email"/>
        <rdfs:comment>This element represents the concept of &apos;email&apos; as used in the capstone project ontology.</rdfs:comment>
        <rdfs:label>email</rdfs:label>
    </owl:DatatypeProperty>
    


    <!-- http://www.semanticweb.org/abc/ontologies/2025/3/untitled-ontology-11#endDate -->

    <owl:DatatypeProperty rdf:about="http://www.semanticweb.org/abc/ontologies/2025/3/untitled-ontology-11#endDate">
        <rdfs:subPropertyOf rdf:resource="http://www.w3.org/2002/07/owl#topDataProperty"/>
        <rdf:type rdf:resource="http://www.w3.org/2002/07/owl#FunctionalProperty"/>
        <rdfs:domain rdf:resource="http://www.semanticweb.org/abc/ontologies/2025/3/untitled-ontology-11#CapstoneProject"/>
        <rdfs:range rdf:resource="http://schema.org/endDate"/>
        <rdfs:comment>This element represents the concept of &apos;endDate&apos; as used in the capstone project ontology.</rdfs:comment>
        <rdfs:label>endDate</rdfs:label>
    </owl:DatatypeProperty>
    


    <!-- http://www.semanticweb.org/abc/ontologies/2025/3/untitled-ontology-11#feedback -->

    <owl:DatatypeProperty rdf:about="http://www.semanticweb.org/abc/ontologies/2025/3/untitled-ontology-11#feedback">
        <rdfs:subPropertyOf rdf:resource="http://www.w3.org/2002/07/owl#topDataProperty"/>
        <rdfs:domain rdf:resource="http://www.semanticweb.org/abc/ontologies/2025/3/untitled-ontology-11#Assessment"/>
        <rdfs:range rdf:resource="http://www.w3.org/2001/XMLSchema#string"/>
        <rdfs:comment>This element represents the concept of &apos;feedback&apos; as used in the capstone project ontology.</rdfs:comment>
        <rdfs:label>feedback</rdfs:label>
    </owl:DatatypeProperty>
    


    <!-- http://www.semanticweb.org/abc/ontologies/2025/3/untitled-ontology-11#fileSize -->

    <owl:DatatypeProperty rdf:about="http://www.semanticweb.org/abc/ontologies/2025/3/untitled-ontology-11#fileSize">
        <rdfs:subPropertyOf rdf:resource="http://www.w3.org/2002/07/owl#topDataProperty"/>
        <rdfs:domain rdf:resource="http://www.semanticweb.org/abc/ontologies/2025/3/untitled-ontology-11#Documentation"/>
        <rdfs:range rdf:resource="http://schema.org/contentSize"/>
        <rdfs:comment>This element represents the concept of &apos;fileSize&apos; as used in the capstone project ontology.</rdfs:comment>
        <rdfs:label>fileSize</rdfs:label>
    </owl:DatatypeProperty>
    


    <!-- http://www.semanticweb.org/abc/ontologies/2025/3/untitled-ontology-11#fileType -->

    <owl:DatatypeProperty rdf:about="http://www.semanticweb.org/abc/ontologies/2025/3/untitled-ontology-11#fileType">
        <rdfs:subPropertyOf rdf:resource="http://www.w3.org/2002/07/owl#topDataProperty"/>
        <rdfs:domain rdf:resource="http://www.semanticweb.org/abc/ontologies/2025/3/untitled-ontology-11#Documentation"/>
        <rdfs:range rdf:resource="http://schema.org/encodingformat"/>
        <rdfs:comment>This element represents the concept of &apos;fileType&apos; as used in the capstone project ontology.</rdfs:comment>
        <rdfs:label>fileType</rdfs:label>
    </owl:DatatypeProperty>
    


    <!-- http://www.semanticweb.org/abc/ontologies/2025/3/untitled-ontology-11#frameSize -->

    <owl:DatatypeProperty rdf:about="http://www.semanticweb.org/abc/ontologies/2025/3/untitled-ontology-11#frameSize">
        <rdfs:domain rdf:resource="http://www.semanticweb.org/abc/ontologies/2025/3/untitled-ontology-11#Video"/>
        <rdfs:range rdf:resource="http://schema.org/videoFrameSize"/>
        <rdfs:comment>This element represents the concept of &apos;frameSize&apos; as used in the capstone project ontology.</rdfs:comment>
        <rdfs:label>frameSize</rdfs:label>
    </owl:DatatypeProperty>
    


    <!-- http://www.semanticweb.org/abc/ontologies/2025/3/untitled-ontology-11#frameworkName -->

    <owl:DatatypeProperty rdf:about="http://www.semanticweb.org/abc/ontologies/2025/3/untitled-ontology-11#frameworkName">
        <rdfs:subPropertyOf rdf:resource="http://www.w3.org/2002/07/owl#topDataProperty"/>
        <rdfs:domain rdf:resource="http://www.semanticweb.org/abc/ontologies/2025/3/untitled-ontology-11#Framework"/>
        <rdfs:range rdf:resource="http://schema.org/softwareFramework"/>
        <rdfs:comment>This element represents the concept of &apos;frameworkName&apos; as used in the capstone project ontology.</rdfs:comment>
        <rdfs:label>frameworkName</rdfs:label>
    </owl:DatatypeProperty>
    


    <!-- http://www.semanticweb.org/abc/ontologies/2025/3/untitled-ontology-11#isFinalSubmission -->

    <owl:DatatypeProperty rdf:about="http://www.semanticweb.org/abc/ontologies/2025/3/untitled-ontology-11#isFinalSubmission">
        <rdfs:subPropertyOf rdf:resource="http://www.w3.org/2002/07/owl#topDataProperty"/>
        <rdfs:domain rdf:resource="http://www.semanticweb.org/abc/ontologies/2025/3/untitled-ontology-11#Documentation"/>
        <rdfs:range rdf:resource="http://www.w3.org/2001/XMLSchema#boolean"/>
        <rdfs:comment>This element represents the concept of &apos;isFinalSubmission&apos; as used in the capstone project ontology.</rdfs:comment>
        <rdfs:label>isFinalSubmission</rdfs:label>
    </owl:DatatypeProperty>
    


    <!-- http://www.semanticweb.org/abc/ontologies/2025/3/untitled-ontology-11#languageUsed -->

    <owl:DatatypeProperty rdf:about="http://www.semanticweb.org/abc/ontologies/2025/3/untitled-ontology-11#languageUsed">
        <rdfs:subPropertyOf rdf:resource="http://www.w3.org/2002/07/owl#topDataProperty"/>
        <rdfs:domain rdf:resource="http://www.semanticweb.org/abc/ontologies/2025/3/untitled-ontology-11#SourceCode"/>
        <rdfs:range rdf:resource="http://schema.org/programmingLanguage"/>
        <rdfs:comment>This element represents the concept of &apos;languageUsed&apos; as used in the capstone project ontology.</rdfs:comment>
        <rdfs:label>languageUsed</rdfs:label>
    </owl:DatatypeProperty>
    


    <!-- http://www.semanticweb.org/abc/ontologies/2025/3/untitled-ontology-11#lastModified -->

    <owl:DatatypeProperty rdf:about="http://www.semanticweb.org/abc/ontologies/2025/3/untitled-ontology-11#lastModified">
        <rdfs:subPropertyOf rdf:resource="http://www.w3.org/2002/07/owl#topDataProperty"/>
        <rdfs:domain rdf:resource="http://www.semanticweb.org/abc/ontologies/2025/3/untitled-ontology-11#Documentation"/>
        <rdfs:range rdf:resource="http://schema.org/dateModified"/>
        <rdfs:comment>This element represents the concept of &apos;lastModified&apos; as used in the capstone project ontology.</rdfs:comment>
        <rdfs:label>lastModified</rdfs:label>
    </owl:DatatypeProperty>
    


    <!-- http://www.semanticweb.org/abc/ontologies/2025/3/untitled-ontology-11#marksObtained -->

    <owl:DatatypeProperty rdf:about="http://www.semanticweb.org/abc/ontologies/2025/3/untitled-ontology-11#marksObtained">
        <rdfs:subPropertyOf rdf:resource="http://www.w3.org/2002/07/owl#topDataProperty"/>
        <rdfs:domain rdf:resource="http://www.semanticweb.org/abc/ontologies/2025/3/untitled-ontology-11#Assessment"/>
        <rdfs:range rdf:resource="http://www.w3.org/2001/XMLSchema#float"/>
        <rdfs:comment>This element represents the concept of &apos;marksObtained&apos; as used in the capstone project ontology.</rdfs:comment>
        <rdfs:label>marksObtained</rdfs:label>
    </owl:DatatypeProperty>
    


    <!-- http://www.semanticweb.org/abc/ontologies/2025/3/untitled-ontology-11#phoneNumber -->

    <owl:DatatypeProperty rdf:about="http://www.semanticweb.org/abc/ontologies/2025/3/untitled-ontology-11#phoneNumber">
        <rdfs:subPropertyOf rdf:resource="http://www.w3.org/2002/07/owl#topDataProperty"/>
        <rdfs:domain rdf:resource="http://www.semanticweb.org/abc/ontologies/2025/3/untitled-ontology-11#Stakeholder"/>
        <rdfs:range rdf:resource="http://schema.org/telephone"/>
        <rdfs:comment>This element represents the concept of &apos;phoneNumber&apos; as used in the capstone project ontology.</rdfs:comment>
        <rdfs:label>phoneNumber</rdfs:label>
    </owl:DatatypeProperty>
    


    <!-- http://www.semanticweb.org/abc/ontologies/2025/3/untitled-ontology-11#posterFormat -->

    <owl:DatatypeProperty rdf:about="http://www.semanticweb.org/abc/ontologies/2025/3/untitled-ontology-11#posterFormat">
        <rdfs:domain rdf:resource="http://www.semanticweb.org/abc/ontologies/2025/3/untitled-ontology-11#Poster"/>
        <rdfs:range rdf:resource="http://schema.org/encodingformat"/>
        <rdfs:comment>This element represents the concept of &apos;posterFormat&apos; as used in the capstone project ontology.</rdfs:comment>
        <rdfs:label>posterFormat</rdfs:label>
    </owl:DatatypeProperty>
    


    <!-- http://www.semanticweb.org/abc/ontologies/2025/3/untitled-ontology-11#projectDescription -->

    <owl:DatatypeProperty rdf:about="http://www.semanticweb.org/abc/ontologies/2025/3/untitled-ontology-11#projectDescription">
        <rdfs:domain rdf:resource="http://www.semanticweb.org/abc/ontologies/2025/3/untitled-ontology-11#CapstoneProject"/>
        <rdfs:range rdf:resource="http://schema.org/description"/>
        <rdfs:comment>This element represents the concept of &apos;projectDescription&apos; as used in the capstone project ontology.</rdfs:comment>
        <rdfs:label>projectDescription</rdfs:label>
    </owl:DatatypeProperty>
    


    <!-- http://www.semanticweb.org/abc/ontologies/2025/3/untitled-ontology-11#projectTitle -->

    <owl:DatatypeProperty rdf:about="http://www.semanticweb.org/abc/ontologies/2025/3/untitled-ontology-11#projectTitle">
        <rdf:type rdf:resource="http://www.w3.org/2002/07/owl#FunctionalProperty"/>
        <rdfs:domain rdf:resource="http://www.semanticweb.org/abc/ontologies/2025/3/untitled-ontology-11#CapstoneProject"/>
        <rdfs:range rdf:resource="http://schema.org/name"/>
        <rdfs:comment>This element represents the concept of &apos;projectTitle&apos; as used in the capstone project ontology.</rdfs:comment>
        <rdfs:label>projectTitle</rdfs:label>
    </owl:DatatypeProperty>
    


    <!-- http://www.semanticweb.org/abc/ontologies/2025/3/untitled-ontology-11#registrationNumber -->

    <owl:DatatypeProperty rdf:about="http://www.semanticweb.org/abc/ontologies/2025/3/untitled-ontology-11#registrationNumber">
        <rdfs:subPropertyOf rdf:resource="http://www.w3.org/2002/07/owl#topDataProperty"/>
        <rdf:type rdf:resource="http://www.w3.org/2002/07/owl#FunctionalProperty"/>
        <rdfs:domain rdf:resource="http://www.semanticweb.org/abc/ontologies/2025/3/untitled-ontology-11#Student"/>
        <rdfs:range rdf:resource="http://schema.org/identifier"/>
        <rdfs:comment>This element represents the concept of &apos;registrationNumber&apos; as used in the capstone project ontology.</rdfs:comment>
        <rdfs:label>registrationNumber</rdfs:label>
    </owl:DatatypeProperty>
    


    <!-- http://www.semanticweb.org/abc/ontologies/2025/3/untitled-ontology-11#score -->

    <owl:DatatypeProperty rdf:about="http://www.semanticweb.org/abc/ontologies/2025/3/untitled-ontology-11#score">
        <rdfs:subPropertyOf rdf:resource="http://www.w3.org/2002/07/owl#topDataProperty"/>
        <rdfs:domain rdf:resource="http://www.semanticweb.org/abc/ontologies/2025/3/untitled-ontology-11#Assessment"/>
        <rdfs:range rdf:resource="http://www.w3.org/2001/XMLSchema#integer"/>
        <rdfs:comment>This element represents the concept of &apos;score&apos; as used in the capstone project ontology.</rdfs:comment>
        <rdfs:label>score</rdfs:label>
    </owl:DatatypeProperty>
    


    <!-- http://www.semanticweb.org/abc/ontologies/2025/3/untitled-ontology-11#stakeholderName -->

    <owl:DatatypeProperty rdf:about="http://www.semanticweb.org/abc/ontologies/2025/3/untitled-ontology-11#stakeholderName">
        <rdfs:subPropertyOf rdf:resource="http://www.w3.org/2002/07/owl#topDataProperty"/>
        <rdfs:domain rdf:resource="http://www.semanticweb.org/abc/ontologies/2025/3/untitled-ontology-11#Stakeholder"/>
        <rdfs:range rdf:resource="http://schema.org/name"/>
        <rdfs:comment>This element represents the concept of &apos;stakeholderName&apos; as used in the capstone project ontology.</rdfs:comment>
        <rdfs:label>stakeholderName</rdfs:label>
    </owl:DatatypeProperty>
    


    <!-- http://www.semanticweb.org/abc/ontologies/2025/3/untitled-ontology-11#stakeholderRole -->

    <owl:DatatypeProperty rdf:about="http://www.semanticweb.org/abc/ontologies/2025/3/untitled-ontology-11#stakeholderRole">
        <rdfs:subPropertyOf rdf:resource="http://www.w3.org/2002/07/owl#topDataProperty"/>
        <rdfs:domain rdf:resource="http://www.semanticweb.org/abc/ontologies/2025/3/untitled-ontology-11#Stakeholder"/>
        <rdfs:range rdf:resource="http://schema.org/roleName"/>
        <rdfs:comment>This element represents the concept of &apos;stakeholderRole&apos; as used in the capstone project ontology.</rdfs:comment>
        <rdfs:label>stakeholderRole</rdfs:label>
    </owl:DatatypeProperty>
    


    <!-- http://www.semanticweb.org/abc/ontologies/2025/3/untitled-ontology-11#startDate -->

    <owl:DatatypeProperty rdf:about="http://www.semanticweb.org/abc/ontologies/2025/3/untitled-ontology-11#startDate">
        <rdfs:subPropertyOf rdf:resource="http://www.w3.org/2002/07/owl#topDataProperty"/>
        <rdf:type rdf:resource="http://www.w3.org/2002/07/owl#FunctionalProperty"/>
        <rdfs:domain rdf:resource="http://www.semanticweb.org/abc/ontologies/2025/3/untitled-ontology-11#CapstoneProject"/>
        <rdfs:range rdf:resource="http://schema.org/startDate"/>
        <rdfs:comment>This element represents the concept of &apos;startDate&apos; as used in the capstone project ontology.</rdfs:comment>
        <rdfs:label>startDate</rdfs:label>
    </owl:DatatypeProperty>
    


    <!-- http://www.semanticweb.org/abc/ontologies/2025/3/untitled-ontology-11#submissionDate -->

    <owl:DatatypeProperty rdf:about="http://www.semanticweb.org/abc/ontologies/2025/3/untitled-ontology-11#submissionDate">
        <rdfs:subPropertyOf rdf:resource="http://www.w3.org/2002/07/owl#topDataProperty"/>
        <rdfs:domain rdf:resource="http://www.semanticweb.org/abc/ontologies/2025/3/untitled-ontology-11#Documentation"/>
        <rdfs:range rdf:resource="http://schema.org/dateSubmitted"/>
        <rdfs:comment>This element represents the concept of &apos;submissionDate&apos; as used in the capstone project ontology.</rdfs:comment>
        <rdfs:label>submissionDate</rdfs:label>
    </owl:DatatypeProperty>
    


    <!-- http://www.semanticweb.org/abc/ontologies/2025/3/untitled-ontology-11#toolLicense -->

    <owl:DatatypeProperty rdf:about="http://www.semanticweb.org/abc/ontologies/2025/3/untitled-ontology-11#toolLicense">
        <rdfs:subPropertyOf rdf:resource="http://www.w3.org/2002/07/owl#topDataProperty"/>
        <rdfs:domain rdf:resource="http://www.semanticweb.org/abc/ontologies/2025/3/untitled-ontology-11#Tools"/>
        <rdfs:range rdf:resource="http://schema.org/license"/>
        <rdfs:comment>This element represents the concept of &apos;toolLicense&apos; as used in the capstone project ontology.</rdfs:comment>
        <rdfs:label>toolLicense</rdfs:label>
    </owl:DatatypeProperty>
    


    <!-- http://www.semanticweb.org/abc/ontologies/2025/3/untitled-ontology-11#toolName -->

    <owl:DatatypeProperty rdf:about="http://www.semanticweb.org/abc/ontologies/2025/3/untitled-ontology-11#toolName">
        <rdfs:subPropertyOf rdf:resource="http://www.w3.org/2002/07/owl#topDataProperty"/>
        <rdfs:domain rdf:resource="http://www.semanticweb.org/abc/ontologies/2025/3/untitled-ontology-11#Tools"/>
        <rdfs:range rdf:resource="http://schema.org/name"/>
        <rdfs:comment>This element represents the concept of &apos;toolName&apos; as used in the capstone project ontology.</rdfs:comment>
        <rdfs:label>toolName</rdfs:label>
    </owl:DatatypeProperty>
    


    <!-- http://www.semanticweb.org/abc/ontologies/2025/3/untitled-ontology-11#toolType -->

    <owl:DatatypeProperty rdf:about="http://www.semanticweb.org/abc/ontologies/2025/3/untitled-ontology-11#toolType">
        <rdfs:subPropertyOf rdf:resource="http://www.w3.org/2002/07/owl#topDataProperty"/>
        <rdfs:domain rdf:resource="http://www.semanticweb.org/abc/ontologies/2025/3/untitled-ontology-11#Tools"/>
        <rdfs:range rdf:resource="http://www.w3.org/2001/XMLSchema#string"/>
        <rdfs:comment>This element represents the concept of &apos;toolType&apos; as used in the capstone project ontology.</rdfs:comment>
        <rdfs:label>toolType</rdfs:label>
    </owl:DatatypeProperty>
    


    <!-- http://www.semanticweb.org/abc/ontologies/2025/3/untitled-ontology-11#toolVersion -->

    <owl:DatatypeProperty rdf:about="http://www.semanticweb.org/abc/ontologies/2025/3/untitled-ontology-11#toolVersion">
        <rdfs:subPropertyOf rdf:resource="http://www.w3.org/2002/07/owl#topDataProperty"/>
        <rdfs:domain rdf:resource="http://www.semanticweb.org/abc/ontologies/2025/3/untitled-ontology-11#Tools"/>
        <rdfs:range rdf:resource="http://schema.org/version"/>
        <rdfs:comment>This element represents the concept of &apos;toolVersion&apos; as used in the capstone project ontology.</rdfs:comment>
        <rdfs:label>toolVersion</rdfs:label>
    </owl:DatatypeProperty>
    


    <!-- http://www.semanticweb.org/abc/ontologies/2025/3/untitled-ontology-11#videoFormat -->

    <owl:DatatypeProperty rdf:about="http://www.semanticweb.org/abc/ontologies/2025/3/untitled-ontology-11#videoFormat">
        <rdfs:domain rdf:resource="http://www.semanticweb.org/abc/ontologies/2025/3/untitled-ontology-11#Video"/>
        <rdfs:range rdf:resource="http://schema.org/encodingformat"/>
        <rdfs:comment>This element represents the concept of &apos;videoFormat&apos; as used in the capstone project ontology.</rdfs:comment>
        <rdfs:label>videoFormat</rdfs:label>
    </owl:DatatypeProperty>
    


    <!-- http://www.semanticweb.org/abc/ontologies/2025/3/untitled-ontology-11#videoQuality -->

    <owl:DatatypeProperty rdf:about="http://www.semanticweb.org/abc/ontologies/2025/3/untitled-ontology-11#videoQuality">
        <rdfs:domain rdf:resource="http://www.semanticweb.org/abc/ontologies/2025/3/untitled-ontology-11#Video"/>
        <rdfs:range rdf:resource="http://schema.org/videoQuality"/>
        <rdfs:comment>This element represents the concept of &apos;videoQuality&apos; as used in the capstone project ontology.</rdfs:comment>
        <rdfs:label>videoQuality</rdfs:label>
    </owl:DatatypeProperty>
    


    <!-- http://www.semanticweb.org/abc/ontologies/2025/3/untitled-ontology-11#weight -->

    <owl:DatatypeProperty rdf:about="http://www.semanticweb.org/abc/ontologies/2025/3/untitled-ontology-11#weight">
        <rdfs:subPropertyOf rdf:resource="http://www.w3.org/2002/07/owl#topDataProperty"/>
        <rdfs:domain rdf:resource="http://www.semanticweb.org/abc/ontologies/2025/3/untitled-ontology-11#Criteria"/>
        <rdfs:range rdf:resource="http://www.w3.org/2001/XMLSchema#decimal"/>
        <rdfs:comment>This element represents the concept of &apos;weight&apos; as used in the capstone project ontology.</rdfs:comment>
        <rdfs:label>weight</rdfs:label>
    </owl:DatatypeProperty>
    


    <!-- 
    ///////////////////////////////////////////////////////////////////////////////////////
    //
    // Classes
    //
    ///////////////////////////////////////////////////////////////////////////////////////
     -->

    


    <!-- http://schema.org/Code -->

    <owl:Class rdf:about="http://schema.org/Code">
        <rdfs:comment>This represents the class Code which we used from schema.org</rdfs:comment>
        <rdfs:label>Code</rdfs:label>
    </owl:Class>
    


    <!-- http://schema.org/Documentation -->

    <owl:Class rdf:about="http://schema.org/Documentation">
        <rdfs:comment>This represents the class Documentation which we used from schema.org</rdfs:comment>
        <rdfs:label>Documentation</rdfs:label>
    </owl:Class>
    


    <!-- http://schema.org/Person -->

    <owl:Class rdf:about="http://schema.org/Person">
        <rdfs:comment>This represents the class Person which we used from schema.org</rdfs:comment>
        <rdfs:label>Person</rdfs:label>
    </owl:Class>
    


    <!-- http://schema.org/Poster -->

    <owl:Class rdf:about="http://schema.org/Poster">
        <rdfs:comment>This represents the class Poster which we used from schema.org</rdfs:comment>
        <rdfs:label>Poster</rdfs:label>
    </owl:Class>
    


    <!-- http://schema.org/Project -->

    <owl:Class rdf:about="http://schema.org/Project">
        <rdfs:comment>This represents the class Project which we used from schema.org</rdfs:comment>
        <rdfs:label>Project</rdfs:label>
    </owl:Class>
    


    <!-- http://schema.org/Review -->

    <owl:Class rdf:about="http://schema.org/Review">
        <rdfs:comment>This represents the class Review which we used from schema.org</rdfs:comment>
        <rdfs:label>Review</rdfs:label>
    </owl:Class>
    


    <!-- http://schema.org/VideoObject -->

    <owl:Class rdf:about="http://schema.org/VideoObject">
        <rdfs:comment>This represents the class VideoObject which we used from schema.org</rdfs:comment>
        <rdfs:label>Video</rdfs:label>
    </owl:Class>
    


    <!-- http://www.semanticweb.org/abc/ontologies/2025/3/untitled-ontology-11#AIModel -->

    <owl:Class rdf:about="http://www.semanticweb.org/abc/ontologies/2025/3/untitled-ontology-11#AIModel">
        <rdfs:subClassOf rdf:resource="http://www.semanticweb.org/abc/ontologies/2025/3/untitled-ontology-11#Tools"/>
        <rdfs:comment>This class represents the concept of &apos;AlModel&apos; in the capstone project ontology.</rdfs:comment>
        <rdfs:label>AIModel</rdfs:label>
    </owl:Class>
    


    <!-- http://www.semanticweb.org/abc/ontologies/2025/3/untitled-ontology-11#Assessment -->

    <owl:Class rdf:about="http://www.semanticweb.org/abc/ontologies/2025/3/untitled-ontology-11#Assessment">
        <rdfs:subClassOf rdf:resource="http://www.semanticweb.org/abc/ontologies/2025/3/untitled-ontology-11#Evaluation"/>
        <rdfs:comment>This class represents the concept of &apos;Assessment&apos; in the capstone project ontology.</rdfs:comment>
        <rdfs:label>Assessment</rdfs:label>
    </owl:Class>
    


    <!-- http://www.semanticweb.org/abc/ontologies/2025/3/untitled-ontology-11#CapstoneProject -->

    <owl:Class rdf:about="http://www.semanticweb.org/abc/ontologies/2025/3/untitled-ontology-11#CapstoneProject">
        <rdfs:subClassOf rdf:resource="http://schema.org/Project"/>
        <rdfs:subClassOf>
            <owl:Restriction>
                <owl:onProperty rdf:resource="http://www.semanticweb.org/abc/ontologies/2025/3/untitled-ontology-11#hasComponent"/>
                <owl:someValuesFrom rdf:resource="http://www.semanticweb.org/abc/ontologies/2025/3/untitled-ontology-11#ProjectComponent"/>
            </owl:Restriction>
        </rdfs:subClassOf>
        <rdfs:subClassOf>
            <owl:Restriction>
                <owl:onProperty rdf:resource="http://www.semanticweb.org/abc/ontologies/2025/3/untitled-ontology-11#hasProcess"/>
                <owl:someValuesFrom rdf:resource="http://www.semanticweb.org/abc/ontologies/2025/3/untitled-ontology-11#Process"/>
            </owl:Restriction>
        </rdfs:subClassOf>
        <rdfs:subClassOf>
            <owl:Restriction>
                <owl:onProperty rdf:resource="http://www.semanticweb.org/abc/ontologies/2025/3/untitled-ontology-11#hasStakeholder"/>
                <owl:someValuesFrom rdf:resource="http://www.semanticweb.org/abc/ontologies/2025/3/untitled-ontology-11#Stakeholder"/>
            </owl:Restriction>
        </rdfs:subClassOf>
        <rdfs:subClassOf>
            <owl:Restriction>
                <owl:onProperty rdf:resource="http://www.semanticweb.org/abc/ontologies/2025/3/untitled-ontology-11#hasTool"/>
                <owl:someValuesFrom rdf:resource="http://www.semanticweb.org/abc/ontologies/2025/3/untitled-ontology-11#Tools"/>
            </owl:Restriction>
        </rdfs:subClassOf>
        <rdfs:subClassOf>
            <owl:Restriction>
                <owl:onProperty rdf:resource="http://www.semanticweb.org/abc/ontologies/2025/3/untitled-ontology-11#endDate"/>
                <owl:qualifiedCardinality rdf:datatype="http://www.w3.org/2001/XMLSchema#nonNegativeInteger">1</owl:qualifiedCardinality>
                <owl:onDataRange rdf:resource="http://schema.org/endDate"/>
            </owl:Restriction>
        </rdfs:subClassOf>
        <rdfs:subClassOf>
            <owl:Restriction>
                <owl:onProperty rdf:resource="http://www.semanticweb.org/abc/ontologies/2025/3/untitled-ontology-11#startDate"/>
                <owl:qualifiedCardinality rdf:datatype="http://www.w3.org/2001/XMLSchema#nonNegativeInteger">1</owl:qualifiedCardinality>
                <owl:onDataRange rdf:resource="http://schema.org/startDate"/>
            </owl:Restriction>
        </rdfs:subClassOf>
        <rdfs:comment>This class represents the concept of &apos;CapstoneProject&apos; in the capstone project ontology.</rdfs:comment>
        <rdfs:label>CapstoneProject</rdfs:label>
    </owl:Class>
    


    <!-- http://www.semanticweb.org/abc/ontologies/2025/3/untitled-ontology-11#Criteria -->

    <owl:Class rdf:about="http://www.semanticweb.org/abc/ontologies/2025/3/untitled-ontology-11#Criteria">
        <rdfs:subClassOf rdf:resource="http://www.semanticweb.org/abc/ontologies/2025/3/untitled-ontology-11#Evaluation"/>
        <rdfs:comment>This class represents the concept of &apos;Criteria&apos; in the capstone project ontology.</rdfs:comment>
        <rdfs:label>Criteria</rdfs:label>
    </owl:Class>
    


    <!-- http://www.semanticweb.org/abc/ontologies/2025/3/untitled-ontology-11#Database -->

    <owl:Class rdf:about="http://www.semanticweb.org/abc/ontologies/2025/3/untitled-ontology-11#Database">
        <rdfs:subClassOf rdf:resource="http://www.semanticweb.org/abc/ontologies/2025/3/untitled-ontology-11#Tools"/>
        <rdfs:comment>This class represents the concept of &apos;Database&apos; in the capstone project ontology.</rdfs:comment>
        <rdfs:label>Database</rdfs:label>
    </owl:Class>
    


    <!-- http://www.semanticweb.org/abc/ontologies/2025/3/untitled-ontology-11#Deliverable -->

    <owl:Class rdf:about="http://www.semanticweb.org/abc/ontologies/2025/3/untitled-ontology-11#Deliverable">
        <rdfs:subClassOf rdf:resource="http://www.semanticweb.org/abc/ontologies/2025/3/untitled-ontology-11#ProjectComponent"/>
        <rdfs:comment>This class represents the concept of &apos;Deliverable&apos; in the capstone project ontology.</rdfs:comment>
        <rdfs:label>Deliverable</rdfs:label>
    </owl:Class>
    


    <!-- http://www.semanticweb.org/abc/ontologies/2025/3/untitled-ontology-11#DesignDocument -->

    <owl:Class rdf:about="http://www.semanticweb.org/abc/ontologies/2025/3/untitled-ontology-11#DesignDocument">
        <rdfs:subClassOf rdf:resource="http://www.semanticweb.org/abc/ontologies/2025/3/untitled-ontology-11#Documentation"/>
        <owl:disjointWith rdf:resource="http://www.semanticweb.org/abc/ontologies/2025/3/untitled-ontology-11#FinalReport"/>
        <rdfs:comment>This class represents the concept of &apos;DesignDocument&apos; in the capstone project ontology.</rdfs:comment>
        <rdfs:label>DesignDocument</rdfs:label>
    </owl:Class>
    


    <!-- http://www.semanticweb.org/abc/ontologies/2025/3/untitled-ontology-11#DevelopmentTool -->

    <owl:Class rdf:about="http://www.semanticweb.org/abc/ontologies/2025/3/untitled-ontology-11#DevelopmentTool">
        <rdfs:subClassOf rdf:resource="http://www.semanticweb.org/abc/ontologies/2025/3/untitled-ontology-11#Tools"/>
        <rdfs:comment>This class represents the concept of &apos;DevelopmentTool&apos; in the capstone project ontology.</rdfs:comment>
        <rdfs:label>DevelopmentTool</rdfs:label>
    </owl:Class>
    


    <!-- http://www.semanticweb.org/abc/ontologies/2025/3/untitled-ontology-11#Documentation -->

    <owl:Class rdf:about="http://www.semanticweb.org/abc/ontologies/2025/3/untitled-ontology-11#Documentation">
        <rdfs:subClassOf rdf:resource="http://schema.org/Documentation"/>
        <rdfs:subClassOf rdf:resource="http://www.semanticweb.org/abc/ontologies/2025/3/untitled-ontology-11#ProjectComponent"/>
        <rdfs:comment>This class represents the concept of &apos;Documentation&apos; in the capstone project ontology.</rdfs:comment>
        <rdfs:label>Documentation</rdfs:label>
    </owl:Class>
    


    <!-- http://www.semanticweb.org/abc/ontologies/2025/3/untitled-ontology-11#Evaluation -->

    <owl:Class rdf:about="http://www.semanticweb.org/abc/ontologies/2025/3/untitled-ontology-11#Evaluation">
        <rdfs:subClassOf rdf:resource="http://schema.org/Review"/>
        <rdfs:subClassOf rdf:resource="http://www.semanticweb.org/abc/ontologies/2025/3/untitled-ontology-11#ProjectComponent"/>
        <rdfs:subClassOf>
            <owl:Restriction>
                <owl:onProperty rdf:resource="http://www.semanticweb.org/abc/ontologies/2025/3/untitled-ontology-11#evaluatesBasedOnCriteria"/>
                <owl:someValuesFrom rdf:resource="http://www.semanticweb.org/abc/ontologies/2025/3/untitled-ontology-11#Criteria"/>
            </owl:Restriction>
        </rdfs:subClassOf>
        <rdfs:comment>This class represents the concept of &apos;Evaluation&apos; in the capstone project ontology.</rdfs:comment>
        <rdfs:label>Evaluation</rdfs:label>
    </owl:Class>
    


    <!-- http://www.semanticweb.org/abc/ontologies/2025/3/untitled-ontology-11#ExternalEvaluator -->

    <owl:Class rdf:about="http://www.semanticweb.org/abc/ontologies/2025/3/untitled-ontology-11#ExternalEvaluator">
        <rdfs:subClassOf rdf:resource="http://www.semanticweb.org/abc/ontologies/2025/3/untitled-ontology-11#Stakeholder"/>
        <rdfs:comment>This class represents the concept of &apos;ExternalEvaluator&apos; in the capstone project ontology.</rdfs:comment>
        <rdfs:label>ExternalEvaluator</rdfs:label>
    </owl:Class>
    


    <!-- http://www.semanticweb.org/abc/ontologies/2025/3/untitled-ontology-11#FacultyMember -->

    <owl:Class rdf:about="http://www.semanticweb.org/abc/ontologies/2025/3/untitled-ontology-11#FacultyMember">
        <rdfs:subClassOf rdf:resource="http://www.semanticweb.org/abc/ontologies/2025/3/untitled-ontology-11#Stakeholder"/>
        <rdfs:comment>This class represents the concept of &apos;FacultyMember&apos; in the capstone project ontology.</rdfs:comment>
        <rdfs:label>FacultyMember</rdfs:label>
    </owl:Class>
    


    <!-- http://www.semanticweb.org/abc/ontologies/2025/3/untitled-ontology-11#FinalReport -->

    <owl:Class rdf:about="http://www.semanticweb.org/abc/ontologies/2025/3/untitled-ontology-11#FinalReport">
        <rdfs:subClassOf rdf:resource="http://www.semanticweb.org/abc/ontologies/2025/3/untitled-ontology-11#Documentation"/>
        <rdfs:comment>This class represents the concept of &apos;FinalReport&apos; in the capstone project ontology.</rdfs:comment>
        <rdfs:label>FinalReport</rdfs:label>
    </owl:Class>
    


    <!-- http://www.semanticweb.org/abc/ontologies/2025/3/untitled-ontology-11#Framework -->

    <owl:Class rdf:about="http://www.semanticweb.org/abc/ontologies/2025/3/untitled-ontology-11#Framework">
        <rdfs:subClassOf rdf:resource="http://www.semanticweb.org/abc/ontologies/2025/3/untitled-ontology-11#Tools"/>
        <rdfs:comment>This class represents the concept of &apos;Framework&apos; in the capstone project ontology.</rdfs:comment>
        <rdfs:label>Framework</rdfs:label>
    </owl:Class>
    


    <!-- http://www.semanticweb.org/abc/ontologies/2025/3/untitled-ontology-11#Implementation -->

    <owl:Class rdf:about="http://www.semanticweb.org/abc/ontologies/2025/3/untitled-ontology-11#Implementation">
        <rdfs:subClassOf rdf:resource="http://www.semanticweb.org/abc/ontologies/2025/3/untitled-ontology-11#Process"/>
        <rdfs:subClassOf>
            <owl:Restriction>
                <owl:onProperty rdf:resource="http://www.semanticweb.org/abc/ontologies/2025/3/untitled-ontology-11#requiresTool"/>
                <owl:someValuesFrom rdf:resource="http://www.semanticweb.org/abc/ontologies/2025/3/untitled-ontology-11#Tools"/>
            </owl:Restriction>
        </rdfs:subClassOf>
        <rdfs:comment>This class represents the concept of &apos;Implementation&apos; in the capstone project ontology.</rdfs:comment>
        <rdfs:label>Implementation</rdfs:label>
    </owl:Class>
    


    <!-- http://www.semanticweb.org/abc/ontologies/2025/3/untitled-ontology-11#Manager -->

    <owl:Class rdf:about="http://www.semanticweb.org/abc/ontologies/2025/3/untitled-ontology-11#Manager">
        <rdfs:subClassOf rdf:resource="http://www.semanticweb.org/abc/ontologies/2025/3/untitled-ontology-11#Stakeholder"/>
        <rdfs:subClassOf>
            <owl:Restriction>
                <owl:onProperty rdf:resource="http://www.semanticweb.org/abc/ontologies/2025/3/untitled-ontology-11#managesProjectComponent"/>
                <owl:someValuesFrom rdf:resource="http://www.semanticweb.org/abc/ontologies/2025/3/untitled-ontology-11#ProjectComponent"/>
            </owl:Restriction>
        </rdfs:subClassOf>
        <rdfs:comment>This class represents the concept of &apos;Manager&apos; in the capstone project ontology.</rdfs:comment>
        <rdfs:label>Manager</rdfs:label>
    </owl:Class>
    


    <!-- http://www.semanticweb.org/abc/ontologies/2025/3/untitled-ontology-11#Planning -->

    <owl:Class rdf:about="http://www.semanticweb.org/abc/ontologies/2025/3/untitled-ontology-11#Planning">
        <rdfs:subClassOf rdf:resource="http://www.semanticweb.org/abc/ontologies/2025/3/untitled-ontology-11#Process"/>
        <rdfs:comment>This class represents the concept of &apos;Planning&apos; in the capstone project ontology.</rdfs:comment>
        <rdfs:label>Planning</rdfs:label>
    </owl:Class>
    


    <!-- http://www.semanticweb.org/abc/ontologies/2025/3/untitled-ontology-11#Poster -->

    <owl:Class rdf:about="http://www.semanticweb.org/abc/ontologies/2025/3/untitled-ontology-11#Poster">
        <rdfs:subClassOf rdf:resource="http://schema.org/Poster"/>
        <rdfs:subClassOf rdf:resource="http://www.semanticweb.org/abc/ontologies/2025/3/untitled-ontology-11#ProjectComponent"/>
        <rdfs:comment>This class represents the concept of &apos;Poster&apos; in the capstone project ontology.</rdfs:comment>
        <rdfs:label>Poster</rdfs:label>
    </owl:Class>
    


    <!-- http://www.semanticweb.org/abc/ontologies/2025/3/untitled-ontology-11#Postertool -->

    <owl:Class rdf:about="http://www.semanticweb.org/abc/ontologies/2025/3/untitled-ontology-11#Postertool">
        <rdfs:subClassOf rdf:resource="http://www.semanticweb.org/abc/ontologies/2025/3/untitled-ontology-11#Tools"/>
        <rdfs:comment>This class represents the concept of &apos;Postertool&apos; in the capstone project ontology.</rdfs:comment>
        <rdfs:label>Postertool</rdfs:label>
    </owl:Class>
    


    <!-- http://www.semanticweb.org/abc/ontologies/2025/3/untitled-ontology-11#Presentation -->

    <owl:Class rdf:about="http://www.semanticweb.org/abc/ontologies/2025/3/untitled-ontology-11#Presentation">
        <rdfs:subClassOf rdf:resource="http://www.semanticweb.org/abc/ontologies/2025/3/untitled-ontology-11#Process"/>
        <rdfs:comment>This class represents the concept of &apos;Presentation&apos; in the capstone project ontology.</rdfs:comment>
        <rdfs:label>Presentation</rdfs:label>
    </owl:Class>
    


    <!-- http://www.semanticweb.org/abc/ontologies/2025/3/untitled-ontology-11#Process -->

    <owl:Class rdf:about="http://www.semanticweb.org/abc/ontologies/2025/3/untitled-ontology-11#Process">
        <rdfs:subClassOf rdf:resource="http://www.semanticweb.org/abc/ontologies/2025/3/untitled-ontology-11#CapstoneProject"/>
        <rdfs:subClassOf>
            <owl:Restriction>
                <owl:onProperty rdf:resource="http://www.semanticweb.org/abc/ontologies/2025/3/untitled-ontology-11#produces"/>
                <owl:someValuesFrom rdf:resource="http://www.semanticweb.org/abc/ontologies/2025/3/untitled-ontology-11#Deliverable"/>
            </owl:Restriction>
        </rdfs:subClassOf>
        <rdfs:subClassOf>
            <owl:Restriction>
                <owl:onProperty rdf:resource="http://www.semanticweb.org/abc/ontologies/2025/3/untitled-ontology-11#useTool"/>
                <owl:someValuesFrom rdf:resource="http://www.semanticweb.org/abc/ontologies/2025/3/untitled-ontology-11#Tools"/>
            </owl:Restriction>
        </rdfs:subClassOf>
        <rdfs:comment>This class represents the concept of &apos;Process&apos; in the capstone project ontology.</rdfs:comment>
        <rdfs:label>Process</rdfs:label>
    </owl:Class>
    


    <!-- http://www.semanticweb.org/abc/ontologies/2025/3/untitled-ontology-11#ProgrammingLanguage -->

    <owl:Class rdf:about="http://www.semanticweb.org/abc/ontologies/2025/3/untitled-ontology-11#ProgrammingLanguage">
        <rdfs:subClassOf rdf:resource="http://www.semanticweb.org/abc/ontologies/2025/3/untitled-ontology-11#Tools"/>
        <rdfs:comment>This element represents the concept of &apos;ProgrammingLanguage&apos; as used in the capstone project ontology.</rdfs:comment>
        <rdfs:label>ProgrammingLanguage</rdfs:label>
    </owl:Class>
    


    <!-- http://www.semanticweb.org/abc/ontologies/2025/3/untitled-ontology-11#ProjectComponent -->

    <owl:Class rdf:about="http://www.semanticweb.org/abc/ontologies/2025/3/untitled-ontology-11#ProjectComponent">
        <rdfs:subClassOf rdf:resource="http://www.semanticweb.org/abc/ontologies/2025/3/untitled-ontology-11#CapstoneProject"/>
        <rdfs:comment>This class represents the concept of &apos;ProjectComponent&apos; in the capstone project ontology.</rdfs:comment>
        <rdfs:label>ProjectComponent</rdfs:label>
    </owl:Class>
    


    <!-- http://www.semanticweb.org/abc/ontologies/2025/3/untitled-ontology-11#Proposal -->

    <owl:Class rdf:about="http://www.semanticweb.org/abc/ontologies/2025/3/untitled-ontology-11#Proposal">
        <rdfs:subClassOf rdf:resource="http://www.semanticweb.org/abc/ontologies/2025/3/untitled-ontology-11#ProjectComponent"/>
        <rdfs:comment>This class represents the concept of &apos;Proposal&apos; in the capstone project ontology.</rdfs:comment>
        <rdfs:label>Proposal</rdfs:label>
    </owl:Class>
    


    <!-- http://www.semanticweb.org/abc/ontologies/2025/3/untitled-ontology-11#Proposaltool -->

    <owl:Class rdf:about="http://www.semanticweb.org/abc/ontologies/2025/3/untitled-ontology-11#Proposaltool">
        <rdfs:subClassOf rdf:resource="http://www.semanticweb.org/abc/ontologies/2025/3/untitled-ontology-11#Tools"/>
        <rdfs:comment>This class represents the concept of &apos;Proposaltool&apos; in the capstone project ontology.</rdfs:comment>
        <rdfs:label>Proposaltool</rdfs:label>
    </owl:Class>
    


    <!-- http://www.semanticweb.org/abc/ontologies/2025/3/untitled-ontology-11#SRS -->

    <owl:Class rdf:about="http://www.semanticweb.org/abc/ontologies/2025/3/untitled-ontology-11#SRS">
        <rdfs:subClassOf rdf:resource="http://www.semanticweb.org/abc/ontologies/2025/3/untitled-ontology-11#Documentation"/>
        <rdfs:comment>This class represents the concept of &apos;SRS&apos; in the capstone project ontology.</rdfs:comment>
        <rdfs:label>SRS</rdfs:label>
    </owl:Class>
    


    <!-- http://www.semanticweb.org/abc/ontologies/2025/3/untitled-ontology-11#SourceCode -->

    <owl:Class rdf:about="http://www.semanticweb.org/abc/ontologies/2025/3/untitled-ontology-11#SourceCode">
        <rdfs:subClassOf rdf:resource="http://schema.org/Code"/>
        <rdfs:subClassOf rdf:resource="http://www.semanticweb.org/abc/ontologies/2025/3/untitled-ontology-11#Deliverable"/>
        <rdfs:comment>This class represents the concept of &apos;SourceCode&apos; in the capstone project ontology.</rdfs:comment>
        <rdfs:label>SourceCode</rdfs:label>
    </owl:Class>
    


    <!-- http://www.semanticweb.org/abc/ontologies/2025/3/untitled-ontology-11#Stakeholder -->

    <owl:Class rdf:about="http://www.semanticweb.org/abc/ontologies/2025/3/untitled-ontology-11#Stakeholder">
        <rdfs:subClassOf rdf:resource="http://schema.org/Person"/>
        <rdfs:subClassOf rdf:resource="http://www.semanticweb.org/abc/ontologies/2025/3/untitled-ontology-11#CapstoneProject"/>
        <rdfs:subClassOf>
            <owl:Restriction>
                <owl:onProperty rdf:resource="http://www.semanticweb.org/abc/ontologies/2025/3/untitled-ontology-11#email"/>
                <owl:qualifiedCardinality rdf:datatype="http://www.w3.org/2001/XMLSchema#nonNegativeInteger">1</owl:qualifiedCardinality>
                <owl:onDataRange rdf:resource="http://schema.org/email"/>
            </owl:Restriction>
        </rdfs:subClassOf>
        <rdfs:comment>This class represents the concept of &apos;Stakeholder&apos; in the capstone project ontology.</rdfs:comment>
        <rdfs:label>Stakeholder</rdfs:label>
    </owl:Class>
    


    <!-- http://www.semanticweb.org/abc/ontologies/2025/3/untitled-ontology-11#Student -->

    <owl:Class rdf:about="http://www.semanticweb.org/abc/ontologies/2025/3/untitled-ontology-11#Student">
        <rdfs:subClassOf rdf:resource="http://www.semanticweb.org/abc/ontologies/2025/3/untitled-ontology-11#Stakeholder"/>
        <rdfs:subClassOf>
            <owl:Restriction>
                <owl:onProperty rdf:resource="http://schema.org/creator"/>
                <owl:someValuesFrom rdf:resource="http://www.semanticweb.org/abc/ontologies/2025/3/untitled-ontology-11#Proposal"/>
            </owl:Restriction>
        </rdfs:subClassOf>
        <rdfs:subClassOf>
            <owl:Restriction>
                <owl:onProperty rdf:resource="http://www.semanticweb.org/abc/ontologies/2025/3/untitled-ontology-11#implementsProcess"/>
                <owl:someValuesFrom rdf:resource="http://www.semanticweb.org/abc/ontologies/2025/3/untitled-ontology-11#Process"/>
            </owl:Restriction>
        </rdfs:subClassOf>
        <rdfs:subClassOf>
            <owl:Restriction>
                <owl:onProperty rdf:resource="http://www.semanticweb.org/abc/ontologies/2025/3/untitled-ontology-11#presentedBy"/>
                <owl:someValuesFrom rdf:resource="http://www.semanticweb.org/abc/ontologies/2025/3/untitled-ontology-11#Presentation"/>
            </owl:Restriction>
        </rdfs:subClassOf>
        <rdfs:subClassOf>
            <owl:Restriction>
                <owl:onProperty rdf:resource="http://www.semanticweb.org/abc/ontologies/2025/3/untitled-ontology-11#submitsTo"/>
                <owl:someValuesFrom rdf:resource="http://www.semanticweb.org/abc/ontologies/2025/3/untitled-ontology-11#Manager"/>
            </owl:Restriction>
        </rdfs:subClassOf>
        <rdfs:subClassOf>
            <owl:Restriction>
                <owl:onProperty rdf:resource="http://www.semanticweb.org/abc/ontologies/2025/3/untitled-ontology-11#registrationNumber"/>
                <owl:qualifiedCardinality rdf:datatype="http://www.w3.org/2001/XMLSchema#nonNegativeInteger">1</owl:qualifiedCardinality>
                <owl:onDataRange rdf:resource="http://schema.org/identifier"/>
            </owl:Restriction>
        </rdfs:subClassOf>
        <rdfs:comment>This class represents the concept of &apos;Student&apos; in the capstone project ontology.</rdfs:comment>
        <rdfs:label>Student</rdfs:label>
    </owl:Class>
    


    <!-- http://www.semanticweb.org/abc/ontologies/2025/3/untitled-ontology-11#Supervisor -->

    <owl:Class rdf:about="http://www.semanticweb.org/abc/ontologies/2025/3/untitled-ontology-11#Supervisor">
        <rdfs:subClassOf rdf:resource="http://www.semanticweb.org/abc/ontologies/2025/3/untitled-ontology-11#Stakeholder"/>
        <rdfs:subClassOf>
            <owl:Restriction>
                <owl:onProperty rdf:resource="http://www.semanticweb.org/abc/ontologies/2025/3/untitled-ontology-11#supervises"/>
                <owl:someValuesFrom rdf:resource="http://www.semanticweb.org/abc/ontologies/2025/3/untitled-ontology-11#Student"/>
            </owl:Restriction>
        </rdfs:subClassOf>
        <rdfs:comment>This class represents the concept of &apos;Supervisor&apos; in the capstone project ontology.</rdfs:comment>
        <rdfs:label>Supervisor</rdfs:label>
    </owl:Class>
    


    <!-- http://www.semanticweb.org/abc/ontologies/2025/3/untitled-ontology-11#Tools -->

    <owl:Class rdf:about="http://www.semanticweb.org/abc/ontologies/2025/3/untitled-ontology-11#Tools">
        <rdfs:subClassOf rdf:resource="http://www.semanticweb.org/abc/ontologies/2025/3/untitled-ontology-11#CapstoneProject"/>
        <rdfs:comment>This class represents the concept of &apos;Tools&apos; in the capstone project ontology.</rdfs:comment>
        <rdfs:label>Tools</rdfs:label>
    </owl:Class>
    


    <!-- http://www.semanticweb.org/abc/ontologies/2025/3/untitled-ontology-11#UserManual -->

    <owl:Class rdf:about="http://www.semanticweb.org/abc/ontologies/2025/3/untitled-ontology-11#UserManual">
        <rdfs:subClassOf rdf:resource="http://www.semanticweb.org/abc/ontologies/2025/3/untitled-ontology-11#Deliverable"/>
        <rdfs:comment>This class represents the concept of &apos;UserManual&apos; in the capstone project ontology.</rdfs:comment>
        <rdfs:label>UserManual</rdfs:label>
    </owl:Class>
    


    <!-- http://www.semanticweb.org/abc/ontologies/2025/3/untitled-ontology-11#Video -->

    <owl:Class rdf:about="http://www.semanticweb.org/abc/ontologies/2025/3/untitled-ontology-11#Video">
        <rdfs:subClassOf rdf:resource="http://schema.org/VideoObject"/>
        <rdfs:subClassOf rdf:resource="http://www.semanticweb.org/abc/ontologies/2025/3/untitled-ontology-11#ProjectComponent"/>
        <rdfs:comment>This class represents the concept of &apos;Video&apos; in the capstone project ontology.</rdfs:comment>
        <rdfs:label>Video</rdfs:label>
    </owl:Class>
    


    <!-- http://www.semanticweb.org/abc/ontologies/2025/3/untitled-ontology-11#Videotool -->

    <owl:Class rdf:about="http://www.semanticweb.org/abc/ontologies/2025/3/untitled-ontology-11#Videotool">
        <rdfs:subClassOf rdf:resource="http://www.semanticweb.org/abc/ontologies/2025/3/untitled-ontology-11#Tools"/>
        <rdfs:comment>This class represents the concept of &apos;Videotool&apos; in the capstone project ontology.</rdfs:comment>
        <rdfs:label>Videotool</rdfs:label>
    </owl:Class>
</rdf:RDF>



<!-- Generated by the OWL API (version 4.5.29.2024-05-13T12:11:03Z) https://github.com/owlcs/owlapi -->

